floyd/VSU_addmain.v
@@ -907,3 +907,20 @@ Ltac MainVSUJoinVSU LP_VSU1 VSU2 :=
 |
 |
 ].
+
+Definition in_dom {A} (T:PTree.t unit) (ia: ident*A) : bool :=
+ match PTree.get (fst ia) T with Some _ => true | None => false end.
+
+Definition mkLinkedSYS_aux (T:PTree.t unit) (p:Clight.program) Specs :funspecs :=
+   filter (in_dom T) (augment_funspecs p Specs).
+
+Definition mkLinkedSYS' (p:Clight.program) Specs :funspecs := 
+  mkLinkedSYS_aux
+  (fold_right (fun i t => PTree.set i tt t) (PTree.empty _) (ExtIDs p)) p Specs.
+(*Do this on per-program basis
+Definition mkLinkedSYS (p:Clight.program) Specs :funspecs := ltac: 
+    (let x := constr:(mkLinkedSYS_aux
+           (fold_right (fun i t => PTree.set i tt t) (PTree.empty _) (ExtIDs p)) p Specs)
+           in let x := eval compute in x
+           in exact x).
+*)
